src/OSum/fundamental.v
@@ -1,0 +1,566 @@
+From stdpp Require Import base gmap coPset tactics proof_irrel.
+
+From iris.base_logic Require Import invariants iprop upred saved_prop gen_heap.
+From iris.base_logic.lib Require Import ghost_map.
+From iris.algebra Require Import cofe_solver gset gmap_view excl.
+From iris.proofmode Require Import proofmode.
+From iris.program_logic Require Import weakestpre ectx_lifting.
+Require Import Autosubst.Autosubst.
+
+From Equations Require Import Equations.
+
+From MyProject.src.OSum Require Export OSum logrel.
+
+
+Fixpoint env_subst (vs : list val) : var → expr :=
+match vs with
+| [] => ids
+| v :: vs' => (of_val v) .: env_subst vs'
+end.
+
+Check interp_env.
+Definition log_typed `{logrelSig Σ} (Γ : list type) (e : expr) (τ : type) : iProp Σ :=
+    (□ ∀ rho (vs : list val), ⟦ Γ ⟧* rho vs -∗ ⟦ τ ⟧ₑ rho e.[env_subst vs])%I.
+
+Notation "Γ ⊨ e : τ" := (log_typed Γ e τ) (at level 74, e, τ at next level).
+
+Module fund.
+  
+    Import OSum.
+
+    Context`{logrelSig Σ}.
+
+    Lemma interp_expr_bind K e Δ τ τ' :
+        ⟦ τ ⟧ₑ Δ e -∗ (∀ v, ⟦ τ ⟧ Δ v -∗ ⟦ τ' ⟧ₑ Δ (fill K (of_val v))) -∗ ⟦ τ' ⟧ₑ Δ (fill K e).
+    Proof.
+        (* Recall interp_expr := (WP e {{ v, ⟦ τ ⟧ rho v }}) *)
+        iIntros.
+        Check wp_bind.
+        (* 
+            wp_bind :=  WP e {{ v, WP (K (of_val v)) {{ v, Φ v }} }} ⊢ WP (K e) {{ v, Φ v }}
+            
+            If goal is a weakest precondition 
+                where the expression is some evaluation context applied to an expressions,
+
+            Then you can factor that into nested weakest preconditions which 
+                first, evaluate the expression e to a value v,
+                second, return the weakest precondition of the evaluation context applied to the 
+                    value v
+        *)
+        iApply wp_bind.
+        (* 
+            Use to adjust the postcondition 
+
+            Lemma wp_wand s E e Φ Ψ :
+                WP e {{ Φ }} -∗ (∀ v, Φ v -∗ Ψ v) -∗ WP e {{ Ψ }}.
+        *)
+        Check wp_wand.
+        iApply (wp_wand with "[$]").
+        done.
+    Qed.
+
+
+    Lemma env_subst_lookup vs x v :
+    vs !! x = Some v → env_subst vs x = of_val v.
+    Proof.
+    revert vs; induction x as [|x IH] => vs.
+    - by destruct vs; inversion 1.
+    - destruct vs as [|w vs]; first by inversion 1.
+        rewrite -lookup_tail /=.
+        apply IH.
+    Qed.
+
+    Lemma sem_typed_var Γ x τ :
+        Γ !! x = Some τ → ⊢ Γ ⊨ Var x : τ.
+    Proof.
+        iIntros (? Δ vs) "!# #HΓ"; simpl.
+        iDestruct (interp_env_Some_l with "HΓ") as (v) "[% ?]"; first done.
+        erewrite env_subst_lookup; eauto.
+        iApply wp_value; done.
+    Qed.
+
+    Lemma sem_typed_case Γ l x τ :
+          Γ !! x = Some (TCase τ) → ⊢ Γ ⊨ Case l : TCase τ.
+    Proof.
+        iIntros (asm rho gamma) "!# #HG".
+        (* case is a value *)
+        iApply wp_value.
+        Check interp_env_Some_l.
+        iDestruct (interp_env_Some_l with "HG") as (v) "[% H]"; first done.
+
+        iDestruct ("H") as "[%l' (H1 & H2)]".
+        iExists l.
+        iSplit. iPureIntro. reflexivity.
+        (* The assumption for this lemma is not strong enough...
+            would have to modify interp_env_Some_l
+            
+            Should we really have this rule anyway? It is for typing dynamic expressions.
+         *)
+       Abort.
+
+
+
+    Lemma sem_typed_unit Γ : ⊢ Γ ⊨ Unit : TUnit.
+    Proof.
+        iIntros (rho gamma) "!# _" .
+        unfold interp_expr.
+        unfold interp.
+        unfold interp_TUnit.
+        simpl.
+        iApply wp_value.
+        done.
+    Qed.
+
+    Lemma sem_typed_int Γ (n : nat) : ⊢ Γ ⊨ #n n : TInt.
+    Proof.
+        iIntros (rho gamma) "!# _".
+        iApply wp_value.
+        iExists n.
+        done.
+    Qed.
+
+    Lemma sem_typed_bool Γ b : ⊢ Γ ⊨ #♭ b : TBool.
+    Proof.
+        iIntros (rho gamma) "!# _".
+        iApply wp_value.
+        iExists b.
+        done.
+    Qed.
+
+    Lemma sem_typed_pair Γ e1 e2 τ1 τ2 :
+        Γ ⊨ e1 : τ1 -∗
+        Γ ⊨ e2 : τ2 -∗
+        Γ ⊨ Pair e1 e2 : TProd τ1 τ2.
+    Proof.
+        iIntros "#H1 #H2" (rho gamma) "!# #HG". simpl.
+        Print PairLCtx.
+        Print fill_item.
+        Print fill.
+        Eval simpl in fill [PairLCtx Unit] Unit. 
+        Check interp_expr_bind [PairLCtx _].
+        (* 
+            ⟦ TProd τ1 τ2 ⟧ₑ rho (Pair e1.[env_subst gamma] e2.[env_subst gamma])
+
+            Here we are interpreting a pair of two expressions e1,e2 according to interp_TProd
+            
+            To break this appart, interp_expr_bind to get the first expression e1 to a value.
+        *)
+        iApply (interp_expr_bind [PairLCtx _ ]).
+        - iApply "H1". done.
+        - iIntros (v1) "#Hv1". simpl.
+        (* 
+            ⟦ TProd τ1 τ2 ⟧ₑ rho (Pair (of_val v) e2.[env_subst gamma])
+
+            Now, work on getting the second expression to a value
+        *)
+        iApply (interp_expr_bind [PairRCtx _ ]).
+        + iApply "H2". done.
+        + iIntros (v2) "#Hv2". simpl.
+        Check interp_expr.
+        (* 
+            ⟦ TProd τ1 τ2 ⟧ₑ rho (Pair (of_val v1) (of_val v2))
+
+            Recall interp_expr := (WP e {{ v, ⟦ τ ⟧ rho v }})
+
+            so the goal is really
+                WP Pair (of_val v1) (of_val v2) {{ v, ⟦ TProd τ1 τ2 ⟧ rho v }}
+
+            and we can use wp_value to dispatch this.
+        *)
+        unfold interp_expr.
+        iApply wp_value.
+        (* 
+            Now we just need to prove the value relation
+            
+            ⟦ TProd τ1 τ2 ⟧ rho (PairV v1 v2)
+
+            Recall interp_TProd  := 
+                λne rho, PersPred(fun v => (∃ v1 v2 , ⌜v = PairV v1 v2⌝  ∗ interp1 rho v1  ∗ interp2 rho v2))%I.  
+        *)
+        simpl.
+        iExists v1. iExists v2.
+        iSplit.
+        {done. }
+        iSplit.
+        { iApply "Hv1". }
+        iApply "Hv2".
+    Qed.
+
+
+    Lemma sem_typed_fst Γ e τ1 τ2 : Γ ⊨ e : TProd τ1 τ2 -∗ Γ ⊨ Fst e : τ1.
+    Proof.
+        iIntros "#HP " (rho gamma) "!# #HG".
+        iSpecialize ("HP" $! rho gamma with "HG").
+        (* use interp_expr_ind to get to a value*)
+        iApply (interp_expr_bind [FstCtx]).
+        - iApply "HP".
+        - iIntros (v) "#HV".
+        (*
+            Now we have some value, v, which is interpreted as a product type. 
+            So we know it should be able to split into a pair of values
+        *)
+        iEval (simpl) in "HV".
+        iDestruct "HV" as "[%v1 [%v2 (%vPair & interp_v1 & interp_v2)]]".
+        subst.
+        (* 
+            now we can show that since v = (v1, v2), fst v = v1
+        *)
+        simpl.
+        iApply wp_pure_step_later; try done.
+        iModIntro. iIntros. iApply wp_value. iApply "interp_v1".
+    Qed.
+
+
+    Lemma sem_typed_snd Γ e τ1 τ2 : Γ ⊨ e : TProd τ1 τ2 -∗ Γ ⊨ Snd e : τ2.
+    Proof.
+        iIntros "#HP " (rho gamma) "!# #HG".
+        iSpecialize ("HP" $! rho gamma with "HG").
+        (* use interp_expr_ind to get to a value*)
+        iApply (interp_expr_bind [SndCtx]).
+        - iApply "HP".
+        - iIntros (v) "#HV".
+        (*
+            Now we have some value, v, which is interpreted as a product type. 
+            So we know it should be able to split into a pair of values
+        *)
+        iEval (simpl) in "HV".
+        iDestruct "HV" as "[%v1 [%v2 (%vPair & interp_v1 & interp_v2)]]".
+        subst.
+        (* 
+            now we can show that since v = (v1, v2), fst v = v1
+        *)
+        simpl.
+        iApply wp_pure_step_later; try done.
+        iModIntro. iIntros. iApply wp_value. iApply "interp_v2".
+    Qed.
+
+
+    (* Do arrow and then try OSum related ones *)
+
+    Lemma sem_typed_lam Γ e τ1 τ2 : τ1 :: Γ ⊨ e : τ2 -∗ Γ ⊨ Lam e : TArrow τ1 τ2.
+    Proof.
+        iIntros "#HP" (rho gamma) "!# #HG". 
+        iSpecialize ("HP" $! rho). (* can't specialize further without a value *)
+        (*  lam is already a value *)
+        iApply wp_value. 
+        (*
+            recall interp_TArrow := 
+
+                λne rho, PersPred(fun v => 
+                    (□ ∀ v', interp1 rho v' → WP App (of_val v) (of_val v') {{ interp2 rho }}))%I. 
+        *)
+        simpl. iModIntro. iIntros (v') "#Hv'".
+        (*  further specialize HP since we have a value *)
+        iSpecialize ("HP" $! (v' :: gamma)).
+
+        (*  Application is a pure step, as we've defined in wp_rules *)
+        Check pure_lam.
+        iApply wp_pure_step_later ; try done.
+        iIntros "!> _". (* discard the later credit *)
+        asimpl. (* autosubst tactic performing substitution *)
+        (* Now we can use our initial assumption *) 
+        iApply "HP".
+        (* at this point, we need to use the assumptions about the contexts *)
+        iApply interp_env_cons.
+        iSplit ; done.
+    Qed.
+
+
+    Lemma sem_typed_app Γ e1 e2 τ1 τ2 : 
+        Γ ⊨ e1 : TArrow τ1 τ2 -∗ 
+        Γ ⊨ e2 : τ1 -∗ 
+        Γ ⊨ App e1 e2 : τ2.
+    Proof.
+        iIntros "#H1 #H2" (rho gamma) "!# #HG".
+        iSpecialize ("H1" $! rho gamma with "HG"). 
+        iSpecialize ("H2" $! rho gamma with "HG"). 
+        (* similar to product, we need to reduce the expressions to values
+        so we can take a step of computation *)
+        Check AppLCtx.
+        iApply (interp_expr_bind [AppLCtx _]).
+        { iApply "H1". }
+        iIntros (v) "HV". simpl.
+        iApply (interp_expr_bind [AppRCtx _]).
+        { iApply "H2". }
+        iIntros (v') "#HV'". simpl.
+        (* all we have to do here is apply HV *)
+        iApply "HV".
+        iApply "HV'".
+    Qed.
+
+    Local Notation "l ↦□ v" := (logrel.pointsto_def l v)
+    (at level 20,  format "l ↦□ v") : bi_scope.
+
+    Lemma sem_typed_osum Γ e1 e2 τ :
+        Γ ⊨ e1 : (TCase τ) -∗
+        Γ ⊨ e2 : τ -∗
+        Γ ⊨ Inj e1 e2 : TOSum.
+    Proof.
+        iIntros "#H1 #H2" (rho gamma) "!# #HG".
+        iSpecialize ("H1" $! rho gamma with "HG"). 
+        iSpecialize ("H2" $! rho gamma with "HG"). 
+        (* reduce both expressions in Inj e1 e2  *)
+        iApply (interp_expr_bind [InjLCtx _]).
+        { iApply "H1". }
+        iIntros (v1) "#HV1". 
+        iApply (interp_expr_bind [InjRCtx _]).
+        { iApply "H2". }
+        iIntros (v2) "#HV2".
+        (* expressions reduced, apply wp_value *)
+        iApply wp_value.
+        (* We have that v1 is a case of τ, so extract that information. *)
+        iDestruct "HV1" as "[%l (%case & #typ)]"; fold interp.
+        subst.
+        (* Now interpret OSum *)
+        iExists l. iExists v2. iExists (interp τ rho).
+        iSplit.
+        iPureIntro. done.
+        iSplit. iApply "typ".
+        iApply "HV2".
+    Qed.
+
+    Lemma points_to_agree l  P P' x : l↦□P -∗ l ↦□ P' -∗ ▷ (P x ≡ P' x).
+    Proof.
+        iIntros "#[%s1 (_ & _ & Q)] #[%s2 (_ & _ & Q')]".
+        iApply (saved_pred_agree with "Q Q'").
+    Qed.
+        
+ 
+    Lemma sem_typed_caseOf  Γ e1 e2 e3 e4 τ1 τ2 : 
+        Γ ⊨ e1 : TOSum -∗ (* thing to destruct *)
+        Γ ⊨ e2 : TCase τ1  -∗ (* matching on case *)
+        τ1  :: Γ ⊨ e3 : τ2  -∗ (* success case *)
+        Γ ⊨ e4 : τ2 -∗ (* failure case *)
+        Γ ⊨ CaseOf e1 e2 e3 e4 : τ2.
+    Proof.
+        iIntros "#H1 #H2 #H3 #H4" (rho gamma) "!# #HG".
+        iSpecialize ("H1" $! rho gamma with "HG"). 
+        iSpecialize ("H2" $! rho gamma with "HG").
+        iSpecialize ("H4" $! rho gamma with "HG").
+        (* evaluate OSum and Case *)
+        iApply (interp_expr_bind [CaseOfCtxOSUM _ _ _]).
+        { iApply "H1". }
+        iIntros (v1) "#HV1". 
+        iApply (interp_expr_bind [CaseOfCtxInj  _ _ _]).
+        { iApply "H2". }
+        iIntros (v2) "#HV2".
+        (* The values of OSum and Case both hold locations, 
+            dispatch redution rules based on the decidable equality of locations *)
+        iDestruct "HV1" as "[%l [%osumVal [%P (%inj & #prf1 & #typ)]]]".
+        iDestruct "HV2" as "[%l' (%case & #prf2)]".
+        subst.
+        fold interp.
+        (* have
+            prf1 : l↦□P
+            prf2 : l'↦□⟦ τ1 ⟧ rho
+            typ : P osumVal
+
+            in the case that l and l' are equal...
+            then P should be equal to interp t1 rho..
+        *)
+        destruct (decide (l = l')) as [|Hneq]. subst.
+        {
+            (*      l'↦□P 
+                AND 
+                    l'↦□⟦ τ1 ⟧ rho 
+                IMPLIES
+                    ▷ (P osumVal ≡ ⟦ τ1 ⟧ rho osumVal) *)
+            iPoseProof (points_to_agree _ _ _ osumVal with "prf1 prf2") as "prf".
+            (* Now we can take a base step, CaseOfTrue  *)
+            iApply wp_pure_step_later ; try done. 
+            (* handle the later modality in goal and hypotheis *)
+            iIntros "!> _". 
+            fold of_val.
+            (* simplify substitutions using autosubst  *)
+            asimpl.
+            (* now we can use our hypothesis about e3 *)
+            iApply ("H3" $! (rho)(osumVal :: gamma)) .
+            (* now we just have to proe the environment interpretation *)
+            iApply interp_env_cons.
+            iSplit.
+            2:{ iApply "HG". }
+            (* use the fact that 
+                P osumVal ≡ ⟦ τ1 ⟧ rho osumVal 
+            *) 
+            iRewrite -"prf".
+            iApply "typ".
+        }
+        iApply wp_pure_step_later.
+        {
+            apply wp_case_nomatch . - unfold AsVal. exists osumVal. reflexivity.
+            - exact Hneq.
+        } eauto.  iIntros "!> _".
+        iApply "H4".
+    Qed.
+(* 
+        Lemma wp_new e v t : 
+        IntoVal e v ->
+        ⊢ WP (New t e) {{ v', True }}.
+(*         {{{ True }}} New t e {{{ v', RET v'; True ∗ True }}}.
+ *)    Proof.
+        intros ev.
+(*         iIntros (phi) "_ HPhi".
+ *)        destruct ev.
+        (* break into the guts WP using using the language lifting *)
+        iApply wp_lift_atomic_base_step_no_fork; auto.
+        iIntros (s1 n k1 k2 n') "#HStinterp".
+        (* get access to the state interpretation *)
+        unfold weakestpre.state_interp; simpl; unfold state_interp.
+
+        (* handle the fact that New is reducible first *)
+        iModIntro. iSplit.
+        - iPureIntro; unfold base_reducible; repeat eexists; eapply NewS.
+        { apply to_of_val. }
+        (* need to show that we can summon a fresh location *)
+        exact (is_fresh s1).
+        - (* now we need to handle the state update, 
+            first bring variables into scope  *)
+        iModIntro. iIntros (e2 s2 efs baseStep) "lc".
+        (* inversion on the base step *)
+        inversion baseStep; subst ; simpl.
+        (*  Show that we can extend state s1 with a fresh location *)
+        assert (s1 ~~> (s1 ∪ {[l]})) as update by done.
+        (* now how do we use that update to modify name_set 
+            using own_update? 
+          first, we only need the ownership under the update modality
+            so use the frame rules to shove things around  
+        *)
+        iApply fupd_frame_l.
+        iSplit. { done. }
+        iApply fupd_frame_r.
+        (* here we need to make a choice w.r.t. the spacial context
+           We dont need HPhi to prove ownership, but we do need it to show
+           that the post condition holds, so push it to that goal  *)
+        iSplitL "HStinterp".
+        (* now we can update the name_set *)
+        {
+            iMod (own_update name_set s1 _ update with "HStinterp");
+            iModIntro ; done. 
+        }
+        rewrite H2. done.
+    Qed. *)
+
+    (* need a Wp lemma about allocation and fresh names *)
+    Lemma sem_typed_new Γ e τ1 τ2 :
+        (TCase τ1) :: Γ ⊨ e : τ2 -∗
+        Γ ⊨ New τ1 e : τ2.
+    Proof.
+        iIntros "#H1" (rho gamma) "!# #HG".
+        unfold interp_expr.
+        iApply wp_lift_atomic_base_step_no_fork; auto.
+        iIntros (s1 n k1 k2 n') "#HStinterp".
+        unfold weakestpre.state_interp; simpl; unfold state_interp.
+
+        Check wp_bind.
+        Check wp_new.
+        iApply wp_wand.
+        { iApply wp_new. admit. }
+        simpl.
+        2:{ 
+        Search wp_bind.
+        iApply wp_new.
+
+
+        (* need a weakest precondition rule fo allocating new types.. *)
+
+
+        (* reduce expression e? *)
+        iApply (interp_expr_bind [NewCtx τ1]).
+        { iApply "H1". }
+    
+
+
+
+(*     Lemma sep_persist (P Q : iProp Sig) { _ : Persistent P}{_ : Persistent Q} : Persistent (P ∗ Q).
+    apply _.
+    Qed.
+
+ (*    Check Forall Persistent.
+    Lemma bigOp_persist (xs : list (iProp Sig))(prfs : Forall Persistent xs) : Persistent ([∗] xs).
+    Proof.
+        induction prfs.
+        - apply _.
+        - unfold Persistent. simpl. iIntros "H".
+        iModIntro. 
+        eapply sep_persist. *)
+        Check big_sepL_persistent_id.
+
+    Check big_opL bi_sep _ _ .
+(*     Notation "'[∗]' Ps" := (big_opL bi_sep (λ _ x, x) Ps%I) : bi_scope.
+ *)
+
+    Local Instance env_persist (Gamma : list type)(gamma : list val)(rho : list D) : Persistent (⟦ Gamma ⟧* rho gamma).
+    Proof.
+        unfold interp_env.
+        eapply sep_persist.
+        - apply _.
+        - eapply big_sepL_persistent_id.
+        Admitted.
+
+
+
+    Check wp_value.
+    Check pure_exec.
+
+    Lemma test : ⊢  WP Unit {{ v, ⌜v = UnitV⌝ }}.
+    Proof.
+        iApply wp_value. done.
+    Qed.
+
+    Lemma test' : True%I  -∗ WP Unit {{ v, ⌜v = UnitV⌝ }}.
+    Proof.
+        iIntros.
+        iApply wp_value.
+        done.
+    Qed.
+
+
+(*     Local Instance unit_exec : PureExec True 1 Unit UnitV.
+ *)    
+    (* notice that without persistant predicates.. 
+        we can only use the fact that gamma satisfies the interpretation in the spacial context
+        go back through the persistent tutorial *)
+    Lemma sem_typed_unit Γ : ⊢ Γ ⊨ Unit : TUnit.
+    Proof.
+        iIntros (rho gamma) "!# _" .
+        unfold interp_expr.
+        unfold interp.
+        unfold interp_TUnit.
+        simpl.
+        iAssert (⌜UnitV = UnitV⌝ %I) as "%H". 
+        - done.
+        -
+        iStopProof.
+        
+        apply wp_value.
+        Locate wp_value.
+        iStopProof.
+        iStartProof.
+        iApply wp_value.
+        simpl.
+        unfold interp_expr.
+        unfold interp.
+        unfold interp_TUnit.
+        iAssert (⌜UnitV = UnitV⌝%I).
+        iPoseProof (wp_value NotStuck empty (fun v => ⌜v = UnitV⌝%I) Unit) as "prf".
+        iApply "prf".
+
+        iApply .
+        simpl.
+        pose proof (wp_value).
+        Locate wp_value.
+        iApply wp_value'.
+        eapply wp_lift_base_step.
+        apply nsteps_once.
+        solve_pure_exec.
+        wp_pure.
+
+        iPoseProof ()
+        unfold wp.
+        unfold wp'.
+
+        Check wp_value.
+        iApply wp_value.
+
+ *)
+End fund.
