src/OSum/logrel.v
@@ -1,0 +1,490 @@
+From stdpp Require Import base gmap coPset tactics proof_irrel.
+
+From iris.base_logic Require Import invariants iprop upred saved_prop gen_heap.
+From iris.base_logic.lib Require Import ghost_map.
+From iris.algebra Require Import cofe_solver gset gmap_view excl.
+From iris.proofmode Require Import proofmode.
+From iris.program_logic Require Import weakestpre.
+Require Import Autosubst.Autosubst.
+
+From Equations Require Import Equations.
+
+From MyProject.src.OSum Require Export OSum persistent_pred wp_rules.
+
+Section logrel.
+(*  we want our semantic domain props to be persistant so they can be duplicated
+ *)
+
+
+    Lemma not_dup (Σ : gFunctors)(P : iProp Σ): P ⊢ P ∗ P.
+    Proof.
+    Fail iIntros "#HP".
+    iIntros "HP".
+    iSplitL.
+    - done.
+    - (* hosed, we already used P *)Abort.
+
+    Lemma pers_dup (Σ : gFunctors)(P : iProp Σ) `{!Persistent P} : P ⊢ P ∗ P.
+    Proof.
+    iIntros "#HP".
+    iSplit.
+    - done.
+    - done.
+    Qed.
+
+
+    Context`{logrelSig Σ}.
+
+    (* do we need to save persistent predicates instead of predicates ..?
+    
+     *)
+    (* 
+    
+    persistent predicates state that the proposition P holds over the sharable parts (core) of the resource
+
+    Local Program Definition uPred_persistently_def {M} (P : uPred M) : uPred M :=
+        {| uPred_holds n x := P n (core x) |}.
+
+
+    Class Persistent {PROP : bi} (P : PROP) := 
+        persistent : P ⊢ □ P.
+
+     *)
+     
+
+
+    Definition D := persistent_pred val (iProp Σ).
+
+    Lemma convert (n : nat)(x y : D) : 
+        @dist_later D (ofe_dist D) n x y -> 
+        @dist_later (val -d> iPropO Σ) (ofe_dist (val -d> iPropO Σ)) n x y.
+    Proof.
+        intros. split. intros. apply H0. exact H1.
+    Qed.
+
+    (*  can I add this to a hint database so solve_proper picks up on it ?
+    https://gitlab.mpi-sws.org/iris/stdpp/-/blob/master/stdpp/tactics.v
+     *)
+    Local Instance saved_persistent_pred_ne (l : loc) : 
+        NonExpansive (λ P : D, saved_pred_own (encode l) DfracDiscarded P).
+    Proof.
+        eapply contractive_ne.
+        red. red. intros.
+        eapply saved_pred_own_contractive.
+        apply convert. 
+        done.
+    Qed.
+
+    Import uPred.
+    Local Program Definition pointsto_def (l : loc) : D -n> iPropO Σ  :=
+        λne P, (∃ (s : state), ⌜l ∈ s⌝ ∗ own name_set s  ∗ saved_pred_own (encode l) (DfracDiscarded) P)%I.
+    Next Obligation.
+        intros l.
+        red. red. intros.
+        eapply uPred_primitive.exist_ne.
+        red. intros s.
+        eapply uPred_primitive.sep_ne.
+        - solve_proper.
+        - eapply uPred_primitive.sep_ne.
+        + solve_proper.
+        + eapply saved_persistent_pred_ne. exact H0.
+    Qed.
+
+
+(*     Local Definition pointsto_def (l : loc)  (P : D) : iProp Σ :=
+        (∃ (s : state), ⌜l ∈ s⌝  ∗ own name_set s  ∗ saved_pred_own (encode l) (DfracDiscarded) P)%I.
+ *)
+
+    (*  why do i have goals of the form  Proper (dist n ==> dist n) ?
+    where is this requirement coming from ? 
+    
+    This is how to state non,expansiveness
+        Notation NonExpansive f := (∀ n, Proper (dist n ==> dist n) f).
+
+        Notation Contractive f := (∀ n, Proper (dist_later n ==> dist n) f).
+
+
+        does being contractive prove being non expansive?
+            have f : X -> Y 
+            ne := forall (n : nat)(x y : X), x ={n}= y -> f x ={n} f y
+
+            contr := forall (n : nat)(x y : X), (forall m < n, x ={m}= y) -> f x ={n}= f y
+
+        yes, proof is here
+            https://plv.mpi-sws.org/coqdoc/iris/iris.algebra.ofe.html#contractive
+
+    *)
+
+    Lemma contrIsNe {X Y : ofe}{f : X -n> Y}(c : Contractive f) : NonExpansive f.
+    Proof.
+        eapply contractive_ne. exact c.
+    Qed.        
+
+
+    Lemma persistant_pred_ne (P : D): NonExpansive P.
+    Proof.
+        solve_proper.
+    Qed.
+          
+    Local Notation "l ↦□ v" := (pointsto_def l v)
+        (at level 20,  format "l ↦□ v") : bi_scope.
+
+    Global Instance mypointsto_persist (l : loc)  (P : D) : Persistent (l ↦□ P).
+    apply _. Qed.
+
+    Definition VRelType := listO D -n> D.
+
+    Program Definition interp_TVar (v : var) : VRelType := 
+        λne rho, PersPred (default (inhabitant : persistent_pred _ _) (rho !! v)).
+    Solve Obligations with repeat intros ?; simpl; solve_proper.
+
+    Program Definition interp_TUnit : VRelType := 
+         λne rho, PersPred(fun v => ⌜v = UnitV⌝%I).
+
+    Definition interp_TInt : VRelType := 
+        λne rho, PersPred(fun v =>(∃ (n : nat), ⌜v = IntV n⌝))%I.
+
+    Definition interp_TBool : VRelType := 
+        λne rho, PersPred(fun v => (∃ (b : bool), ⌜v = BoolV b⌝))%I.
+
+    Program Definition interp_TProd (interp1 interp2 : VRelType) : VRelType := 
+        λne rho, PersPred(fun v => (∃ v1 v2 , ⌜v = PairV v1 v2⌝  ∗ interp1 rho v1  ∗ interp2 rho v2))%I.  
+    Solve Obligations with solve_proper.
+
+    Definition interp_TCase' (interp : VRelType)(rho : listO D) : D :=
+        PersPred(fun v => (∃ l, ⌜v = CaseV l⌝ ∗ l ↦□ (interp rho)))%I.
+
+    Local Instance interp_TCase'_ne (interp : VRelType)(rho : listO D)  : 
+        NonExpansive (PersPred(fun v => (∃ l, ⌜v = CaseV l⌝ ∗ l ↦□ (interp rho)))%I).
+    Proof.        
+        eapply persistant_pred_ne.
+    Qed.
+
+
+    Check persistent_pred_car_ne val (iProp Σ) 0 (interp_TCase' _ _ )(interp_TCase' _ _ ) _ _  _ _. 
+        
+    Program Definition interp_TCase (interp : VRelType) : VRelType := 
+         λne rho, interp_TCase' interp rho.
+    Next Obligation.
+        intro.
+        red. red. intros.
+        try rewrite persistent_pred_ext.
+        pose proof (interp_TCase'_ne interp x ).
+        pose proof (interp_TCase'_ne interp y ).
+        pose proof (persistent_pred_car_ne val (iProp Σ) n (interp_TCase' interp x )(interp_TCase' interp y ) ).
+    Admitted.
+     
+
+
+    Program Definition interp_TOSum : VRelType := 
+        λne rho, PersPred(fun v =>(∃ l v' P , ⌜v = InjV (CaseV l) v'⌝ ∗ l ↦□ P ∗ P v'))%I.
+
+    (* what if state is modified ? *)
+    Program Definition interp_TArrow (interp1 interp2 : VRelType) : VRelType := 
+        λne rho, PersPred(fun v => 
+            (□ ∀ v', interp1 rho v' → WP App (of_val v) (of_val v') {{ interp2 rho }}))%I.
+    Next Obligation.
+        intros i1 i2. solve_proper.
+    Qed.
+
+    (* normal forall, not fresh forall
+       for fresh forall, would need to update saved predicate map? *)
+    Program Definition interp_TForall (interp : VRelType) : VRelType := 
+        λne rho, PersPred(fun v => 
+            (□ ∀ τi : D, WP TApp (of_val v) {{ interp (τi :: rho) }}))%I.
+    Next Obligation.
+        intros i1. solve_proper.
+    Qed.
+
+    Program Definition interp_TExist (interp : VRelType) : VRelType := 
+        λne rho, PersPred(fun v => 
+            (∃ (τi : D) v' ,  ⌜v = PackV v'⌝ ∗ interp (τi :: rho) v))%I.
+    Next Obligation.
+        intros i1. solve_proper.
+    Qed.
+
+    Fixpoint interp (τ : type) : listO D -n> D :=
+        match τ return _ with
+        | TUnit => interp_TUnit
+        | TInt => interp_TInt
+        | TBool => interp_TBool
+        | TProd τ1 τ2 => interp_TProd (interp τ1) (interp τ2)
+        | TArrow τ1 τ2 => interp_TArrow (interp τ1) (interp τ2)
+        | TVar x => interp_TVar x
+        | TForall τ' => interp_TForall (interp τ')
+        | TExist τ' => interp_TExist (interp τ')
+        | TOSum => interp_TOSum
+        | TCase t => interp_TCase (interp t)
+        end.
+    Notation "⟦ τ ⟧" := (interp τ).
+
+    Definition interp_env (Γ : list type)
+        (Δ : list D) (vs : list val) : iProp Σ :=
+        (⌜length Γ = length vs⌝ ∗ [∗] zip_with (λ τ, ⟦ τ ⟧ Δ) Γ vs)%I.
+    Notation "⟦ Γ ⟧*" := (interp_env Γ).
+
+    Global Instance interp_env_base_persistent Δ Γ vs :
+    TCForall Persistent (zip_with (λ τ, ⟦ τ ⟧ Δ) Γ vs).
+    Proof. revert vs; induction Γ => vs; destruct vs; constructor; apply _. Qed.
+    Global Instance interp_env_persistent Γ Δ vs : Persistent (⟦ Γ ⟧* Δ vs) := _.
+
+
+    Lemma interp_env_nil Δ : ⊢ ⟦ [] ⟧* Δ [].
+    Proof. iSplit; simpl; auto. Qed.
+
+    Import uPred.
+    Lemma interp_env_cons Δ Γ vvs τ vv :
+        ⟦ τ :: Γ ⟧* Δ (vv :: vvs) ⊣⊢ ⟦ τ ⟧ Δ vv ∗ ⟦ Γ ⟧* Δ vvs.
+    Proof.
+        rewrite /interp_env /= (assoc _ (⟦ _ ⟧ _ _)) -(comm _ ⌜(_ = _)⌝%I) -assoc.
+        by apply sep_proper; [apply pure_proper; lia|].
+    Qed.
+
+
+    Definition interp_expr (τ : type) (rho : list D) (e : expr) : iProp Σ :=
+        WP e {{ ⟦ τ ⟧ rho }}%I.
+
+    Notation "⟦ τ ⟧ₑ" := (interp_expr τ).
+
+  Lemma interp_env_length Δ Γ vs : ⟦ Γ ⟧* Δ vs ⊢ ⌜length Γ = length vs⌝.
+  Proof. by iIntros "[% ?]". Qed.
+
+  Lemma interp_env_Some_l Δ Γ vs x τ :
+    Γ !! x = Some τ → ⟦ Γ ⟧* Δ vs ⊢ ∃ v, ⌜vs !! x = Some v⌝ ∧ ⟦ τ ⟧ Δ v.
+  Proof.
+    iIntros (?) "[Hlen HΓ]"; iDestruct "Hlen" as %Hlen.
+    destruct (lookup_lt_is_Some_2 vs x) as [v Hv].
+    { by rewrite -Hlen; apply lookup_lt_Some with τ. }
+    iExists v; iSplit; first done. iApply (big_sepL_elem_of with "HΓ").
+    apply elem_of_list_lookup_2 with x.
+    rewrite lookup_zip_with; by simplify_option_eq.
+  Qed.
+
+
+
+    Check upn.
+    Eval compute in upn 2 Var 9. 
+    Check ren.
+
+
+     Lemma interp_weaken Δ1 Π Δ2 τ :
+    ⟦ τ.[upn (length Δ1) (ren (+ length Π))] ⟧ (Δ1 ++ Π ++ Δ2)
+    ≡ ⟦ τ ⟧ (Δ1 ++ Δ2).
+  Proof.
+    revert Δ1 Π Δ2. induction τ=> Δ1 Π Δ2; simpl; auto; intros ?; simpl.
+    - by repeat (f_equiv; try match goal with IH : ∀ _, _ |- _ => by apply IH end).
+    - by repeat (f_equiv; try match goal with IH : ∀ _, _ |- _ => by apply IH end).
+    Admitted.
+(*     - by repeat (f_equiv; try match goal with IH : ∀ _, _ |- _ => by apply IH end).
+    - f_equiv.
+      apply fixpoint_proper=> τi w /=.
+      by repeat (f_equiv; try match goal with IH : ∀ _, _ |- _ => by apply (IH (_ :: _)) end).
+    - rewrite iter_up; destruct lt_dec as [Hl | Hl]; simpl.
+      { by rewrite !lookup_app_l. }
+      rewrite !lookup_app_r; [|lia ..]; do 3 f_equiv; lia.
+    - by repeat (f_equiv; try match goal with IH : ∀ _, _ |- _ => by apply (IH (_ :: _)) end).
+    - by repeat (f_equiv; try match goal with IH : ∀ _, _ |- _ => by apply (IH (_ :: _)) end).
+    - by repeat (f_equiv; try match goal with IH : ∀ _, _ |- _ => by apply IH end).
+  Qed. *)
+
+  Lemma interp_subst_up Δ1 Δ2 τ τ' :
+    ⟦ τ ⟧ (Δ1 ++ interp τ' Δ2 :: Δ2)
+    ≡ ⟦ τ.[upn (length Δ1) (τ' .: ids)] ⟧ (Δ1 ++ Δ2).
+  Proof.
+    revert Δ1 Δ2; induction τ=> Δ1 Δ2; simpl; auto; intros ?; simpl.
+    - by repeat (f_equiv; try match goal with IH : ∀ _, _ |- _ => by apply IH end).
+    - by repeat (f_equiv; try match goal with IH : ∀ _, _ |- _ => by apply IH end).
+    Admitted. (* by repeat (f_equiv; try match goal with IH : ∀ _, _ |- _ => by apply IH end).
+    - f_equiv.
+      apply fixpoint_proper=> τi w /=.
+      by repeat (f_equiv; try match goal with IH : ∀ _, _ |- _ => by apply (IH (_ :: _)) end).
+    - match goal with |- context [_ !! ?x] => rename x into idx end.
+      rewrite iter_up; destruct lt_dec as [Hl | Hl]; simpl.
+      { by rewrite !lookup_app_l. }
+      rewrite !lookup_app_r; [|lia ..].
+      case EQ: (idx - length Δ1) => [|n]; simpl.
+      { symmetry. asimpl. apply (interp_weaken [] Δ1 Δ2 τ'). }
+      rewrite !lookup_app_r; [|lia ..]. do 3 f_equiv. lia.
+    - by repeat (f_equiv; try match goal with IH : ∀ _, _ |- _ => by apply (IH (_ :: _)) end).
+    - by repeat (f_equiv; try match goal with IH : ∀ _, _ |- _ => by apply (IH (_ :: _)) end).
+    - by repeat (f_equiv; try match goal with IH : ∀ _, _ |- _ => by apply IH end).
+  Qed. *)
+
+  Lemma interp_subst Δ2 τ τ' v : ⟦ τ ⟧ (⟦ τ' ⟧ Δ2 :: Δ2) v ≡ ⟦ τ.[τ'/] ⟧ Δ2 v.
+ Admitted.
+    
+
+End logrel.
+
+Global Typeclasses Opaque interp_env.
+Notation "⟦ τ ⟧" := (interp τ).
+Notation "⟦ τ ⟧ₑ" := (interp_expr τ).
+Notation "⟦ Γ ⟧*" := (interp_env Γ).
+
+
+(* 
+
+
+
+    (*  what is the core of our resouce ... 
+
+    Local Instance dfrac_pcore_instance : PCore dfrac := λ dq,
+        match dq with
+        | DfracOwn q ⇒ None
+        | DfracDiscarded ⇒ Some DfracDiscarded
+        | DfracBoth q ⇒ Some DfracDiscarded
+        end.
+    
+
+    what is the meaning of discarded... 
+    
+    Global Instance saved_pred_discarded_persistent γ Φ :
+        Persistent (saved_pred_own γ DfracDiscarded Φ).
+    Proof. apply _. Qed.
+
+    Do I need to say it owns it, or can it just be discarded knowledge ...
+        
+    *)
+
+    (* pure things are always persistent *)
+    Definition p1 (l : loc) : iProp Σ := (∃ (s : state), ⌜l ∈ s⌝)%I.
+    Local Instance pers_p1 (l : loc) : Persistent (p1 l).
+    Proof.
+        apply _.
+    Qed.
+
+    (*  note that
+    
+        Class CoreId {A : cmra} (x : A) := core_id : pcore x ≡ Some x.
+
+        Global Instance own_core_persistent γ a : CoreId a → Persistent (own γ a).
+        Proof. rewrite !own_eq /own_def; apply _. Qed.
+
+        recall, state := gset loc
+
+        hmm.. probably not where the instance is summoned from 
+     *)
+
+    Definition p2 : iProp Σ := (∃ (s : state), own name_set s )%I.
+    Local Instance pers_p2 : Persistent p2.
+    Proof.
+        apply _.
+    Qed.
+
+    Definition p1p2 (l : loc):  iProp Σ := (∃ (s : state), ⌜l ∈ s⌝ ∗ own name_set s )%I.
+    Local Instance pers_p1p2 (l : loc) : Persistent (p1p2 l).
+    apply _. Qed.
+
+
+    Definition p3 (l : loc)  (P : D) : iProp Σ :=  (saved_pred_own (encode l) (DfracOwn 1) P)%I.
+
+    Local Instance pers_p3 (l : loc)  (P : D) : Persistent (p3 l P).
+    Fail apply _.
+    Abort.
+   
+    Definition p3' (l : loc)  (P : D) : iProp Σ :=  (saved_pred_own (encode l) (DfracDiscarded) P)%I.
+    Local Instance pers_p3' (l : loc)  (P : D) : Persistent (p3' l P).
+    apply _. Qed.
+
+
+    (*  Global Instance saved_pred_discarded_persistent γ Φ :
+            Persistent (saved_pred_own γ DfracDiscarded Φ).
+        Proof. apply _. Qed. 
+
+
+        do the saved predicates need to be owned ...?
+
+
+        See this note on the persistent pointsto predicate from the tutorial (persistently.v)
+                    (**
+            Let us now turn to the `discarded' part. If one owns a fraction of a
+            points-to predicate, one can decide to _discard_ the fraction. This
+            means that it is no longer possible to recombine points-to predicates
+            to get the full fraction. As such, the value in the points-to
+            predicate can never be changed again – the location has become
+            read-only. We write [l ↦□ v] for a points-to predicate whose fraction
+            has been discarded. As the [□] suggests, this predicate is persistent.
+            Persistent points-to predicates are great if your program has a
+            read-only location, as it becomes trivial to give all threads access
+            to the associated points-to predicate, and it ensures that no thread
+            can sneakily update the location.
+
+            The [pointsto_persist] lemma asserts that we can update any points-to
+            predicate [l ↦{dq} v] into a persistent one [l ↦□ v].
+            *)
+    *)
+    
+
+
+    Local Instance isIt (l : loc)(P : D) : Persistent (l ↦ P).
+    Proof.
+        unfold Persistent.
+        unfold pointsto_def.
+        unfold bi_persistently.
+        eexists.
+        intros.
+
+
+        r
+        inversion  H1.
+        unfold uPred_holds. simpl. red. red.
+
+    Admitted.
+
+
+
+
+
+   Definition D := val -> iProp Σ.
+
+    Definition VRelType := list D -> D.
+
+    Definition interp_TVar (v : var) : VRelType := 
+        fun rho => (default (fun _ => True%I) (rho !! v)) .
+
+    Definition interp_TUnit : VRelType := 
+        fun rho v => ⌜v = UnitV⌝%I.
+
+    Definition interp_TInt : VRelType := 
+        fun rho v => (∃ (n : nat), ⌜v = IntV n⌝)%I.
+
+    Definition interp_TBool : VRelType := 
+        fun rho v => (∃ (b : bool), ⌜v = BoolV b⌝)%I.
+
+    Definition interp_TProd (interp1 interp2 : VRelType) : VRelType := 
+        fun rho v => (∃ v1 v2 , ⌜v = PairV v1 v2⌝  ∗ interp1 rho v1  ∗ interp2 rho v2)%I.
+
+    Definition interp_TCase (interp : VRelType) : VRelType := 
+        fun rho v => (∃ l, ⌜v = CaseV l⌝ ∗ l ↦ (interp rho))%I.
+
+    Definition interp_TOSum : VRelType := 
+        fun rho v => (∃ l v' P , ⌜v = InjV (CaseV l) v'⌝ ∗ l ↦ P ∗ P v')%I.
+
+    (* what if state is modified ? *)
+    Definition interp_TArrow (interp1 interp2 : VRelType) : VRelType := 
+        fun rho v => (□ ∀ v', interp1 rho v' →
+                        WP App (of_val v) (of_val v') {{ interp2 rho }})%I.
+
+    (* normal forall, not fresh forall
+       for fresh forall, would need to update saved predicate map? *)
+    Definition interp_TForall (interp : VRelType) : VRelType := 
+        fun rho v => (□ ∀ τi : D, WP TApp (of_val v) {{ interp (τi :: rho) }})%I.
+
+    Definition interp_TExist (interp : VRelType) : VRelType := 
+        fun rho v => (∃ (τi : D) v' ,  ⌜v = PackV v'⌝ ∗ interp (τi :: rho) v)%I.
+
+
+    Fixpoint interp (τ : type) : list D -> D :=
+        match τ return _ with
+        | TUnit => interp_TUnit
+        | TInt => interp_TInt
+        | TBool => interp_TBool
+        | TProd τ1 τ2 => interp_TProd (interp τ1) (interp τ2)
+        | TArrow τ1 τ2 => interp_TArrow (interp τ1) (interp τ2)
+        | TVar x => interp_TVar x
+        | TForall τ' => interp_TForall (interp τ')
+        | TExist τ' => interp_TExist (interp τ')
+        | TOSum => interp_TOSum
+        | TCase t => interp_TCase (interp t)
+        end.
+ *)
