src/OSum/wp_rules.v
@@ -1,0 +1,255 @@
+
+From iris.program_logic Require Export weakestpre.
+From iris.program_logic Require Import ectx_lifting.
+From iris.base_logic Require Export invariants saved_prop .
+From iris.algebra Require Import gset.
+From iris.proofmode Require Import proofmode.
+From iris.prelude Require Import options.
+
+Require Import Autosubst.Autosubst.
+
+From MyProject.src.OSum Require Export OSum.
+
+Class logrelSig  Σ := Resources {
+    invariants : invGS Σ;
+    predicates :: savedPredG Σ val ;
+    names :: inG Σ (gsetR loc) ;
+    name_set : gname
+}.
+
+Definition state_interp `{logrelSig Σ} (s : gset loc) : iProp Σ :=
+    own name_set s.
+
+Global Instance OSum_irisGS `{logrelSig Σ} : irisGS OSum_lang Σ := {
+    iris_invGS := invariants;
+    num_laters_per_step _ := 0;
+    state_interp s  _ _ _ := state_interp s;(* gen_heap_interp s; *)
+    fork_post _ := True%I;
+    state_interp_mono _ _ _ _ := fupd_intro _ _
+}.
+
+Section lang_rules.
+    Context `{logrelSig Σ}.
+
+    (*  All of the following is adopted from 
+        A Logical Approach to Type Soundndess 
+        
+
+        Where this stuff comes into play is using rules like
+            wp_pure_step_later    
+            the obligations can be automatically dispatched 
+                by adding the following hints to the database
+
+        This helps avoid breaking into the lower level lemmas such as
+            wp_lift_pure_det_base_step_no_fork 
+    *)
+
+    Ltac inv_base_step :=
+        repeat match goal with
+        | _ => progress simplify_map_eq/= (* simplify memory stuff *)
+        | H : to_val _ = Some _ |- _ => apply of_to_val in H
+        | H : _ = of_val ?v |- _ =>
+            is_var v; destruct v; first[discriminate H|injection H as H]
+        | H : base_step ?e _ _ _ _ _ |- _ =>
+            try (is_var e; fail 1); (* inversion yields many goals if [e] is a variable
+            and can thus better be avoided. *)
+            inversion H; subst; clear H
+        end.
+
+(*     Local Hint Extern 0 (atomic _) => solve_atomic : core.*)
+    Local Hint Extern 0 (base_reducible _ _) => eexists _, _, _, _; simpl : core.
+
+    Local Hint Constructors base_step : core.
+
+    Local Hint Resolve to_of_val : core.
+
+
+    Local Ltac solve_exec_safe :=
+        intros; subst; do 3 eexists; econstructor; simpl; eauto.
+
+    Local Ltac solve_exec_puredet :=
+        simpl; intros;
+        by inv_base_step;
+        repeat match goal with
+            |- context [bool_decide ?A] =>
+                destruct (decide A);
+                [rewrite (bool_decide_eq_true_2 A); last done|
+                rewrite (bool_decide_eq_false_2 A); last done]
+            end; simplify_eq/=; auto.
+    Local Ltac solve_pure_exec :=
+        unfold IntoVal in *;
+        repeat match goal with H : AsVal _ |- _ => destruct H as [??] end; subst;
+        intros ?; apply nsteps_once, pure_base_step_pure_step;
+        constructor; [solve_exec_safe | solve_exec_puredet].
+
+    Global Instance pure_lam e1 e2 `{!AsVal e2} :
+        PureExec True 1 (App (Lam e1) e2) e1.[e2 /].
+    Proof. solve_pure_exec. Qed.
+
+    Global Instance pure_tlam e : PureExec True 1 (TApp (TLam e)) e.
+    Proof. solve_pure_exec. Qed.
+
+    Global Instance pure_pack e1 `{!AsVal e1} e2:
+        PureExec True 1 (UnpackIn (Pack e1) e2) e2.[e1/].
+    Proof. solve_pure_exec. Qed.
+
+    Global Instance pure_fst e1 e2 `{!AsVal e1, !AsVal e2} :
+        PureExec True 1 (Fst (Pair e1 e2)) e1.
+    Proof. solve_pure_exec. Qed.
+
+    Global Instance pure_snd e1 e2 `{!AsVal e1, !AsVal e2} :
+        PureExec True 1 (Snd (Pair e1 e2)) e2.
+    Proof. solve_pure_exec. Qed.
+
+
+    Global Instance wp_if_true e1 e2 :
+        PureExec True 1 (If (#♭ true) e1 e2) e1.
+    Proof. solve_pure_exec. Qed.
+
+    Global Instance wp_if_false e1 e2 :
+        PureExec True 1 (If (#♭ false) e1 e2) e2.
+    Proof. solve_pure_exec. Qed.
+
+    Global Instance wp_int_binop op a b :
+        PureExec True 1 (BinOp op (#n a) (#n b)) (of_val (int_binop_eval op a b)).
+    Proof. destruct op; solve_pure_exec. Qed.
+
+    Global Instance wp_Eq_binop `{!AsVal e1} `{!AsVal e2} :
+        PureExec True 1 (BinOp Eq e1 e2) (#♭ (bool_decide (e1 = e2))).
+    Proof. solve_pure_exec. Qed.
+
+    Global Instance wp_case_match  l `{!AsVal e2} (e3 e4 : expr)  : 
+        PureExec True 1 (CaseOf (Inj (Case l) e2) (Case l) e3 e4) e3.[e2/].
+    Proof. unfold PureExec. intros _.
+        destruct AsVal0. subst.
+        apply nsteps_once. apply pure_base_step_pure_step.
+        constructor.
+        {
+            intros. repeat eexists. eapply CaseOfTrue. - apply to_of_val.
+            - reflexivity.
+        }
+        intros.
+        inversion H0 ; subst.
+        { repeat (try split ; try reflexivity). } 
+        exfalso.
+        pose proof (H12 eq_refl). done.
+    Qed.
+
+    Global Instance wp_case_nomatch l l' `{!AsVal e2} (e3 e4 : expr)  : 
+        l <> l' -> PureExec True 1 (CaseOf (Inj (Case l) e2) (Case l') e3 e4) e4.
+    Proof. unfold PureExec. intros ll _.
+        destruct AsVal0. subst.
+        apply nsteps_once. apply pure_base_step_pure_step.
+        constructor.
+        {
+            intros. repeat eexists. eapply CaseOfFalse. - apply to_of_val.
+            - exact ll.
+        }
+        intros.
+        inversion H0. 
+        { repeat (try split ; try reflexivity). exfalso. pose proof (ll H12). done. } 
+         repeat (try split ; try reflexivity).
+    Qed.
+
+
+    Check gset_disj_alloc_updateP'.
+    Check own_update.
+
+(*     Lemma test (g : gname)(s : gset loc): own g s ⊢ |={⊤}=> own g s.
+    Proof.
+        iIntros "H".
+        assert (s ~~> s).
+        - done.
+        -
+        Check own_update.
+        Fail iMod (own_update $! H0).
+        Abort. *)
+
+(* https://plv.mpi-sws.org/coqdoc/iris/iris.heap_lang.locations.html#Loc.fresh *)
+(*   Definition fresh (ls : gset loc) : loc :=
+    {| loc_car := set_fold (λ k r, (1 + loc_car k) `max` r) 1 ls |}.
+
+  Lemma fresh_fresh ls i : 0 ≤ i → fresh ls +ₗ i ∉ ls.
+  Proof.
+    intros Hi. cut (∀ l, l ∈ ls → loc_car l < loc_car (fresh ls) + i).
+    { intros help Hf%help. simpl in ×. lia. }
+    apply (set_fold_ind_L (λ r ls, ∀ l, l ∈ ls → (loc_car l < r + i)));
+      set_solver by eauto with lia.
+  Qed. *)
+
+  (* vs 
+    stdpp.base.fresh
+   *)
+
+   Lemma fancyToBasic (P : iProp Σ ) : ⊢ (|==> P -∗ |={⊤}=> P)%I.
+   Proof.
+    iIntros.
+    iModIntro.
+    iIntros "HP".
+    iModIntro. 
+    iApply "HP".
+    Qed.
+
+    Lemma sub (s s' : state)(upd : s ~~> s') : own name_set s ⊢ |={⊤}=> own name_set s'.
+    Proof.
+        iIntros "H". 
+        iMod (own_update name_set s s' upd with "H") as "H'".
+        iModIntro. done.
+    Qed.
+(* WP (Case l).[env_subst gamma] {{ v, ⟦ TCase τ ⟧ rho v }}
+ *)
+(*     Lemma wp_new e v t : 
+        IntoVal e v ->
+        ⊢ WP (New t e) {{ v', True }}.
+(*         {{{ True }}} New t e {{{ v', RET v'; True ∗ True }}}.
+ *)    Proof.
+        intros ev.
+(*         iIntros (phi) "_ HPhi".
+ *)        destruct ev.
+        (* break into the guts WP using using the language lifting *)
+        iApply wp_lift_atomic_base_step_no_fork; auto.
+        iIntros (s1 n k1 k2 n') "#HStinterp".
+        (* get access to the state interpretation *)
+        unfold weakestpre.state_interp; simpl; unfold state_interp.
+
+        (* handle the fact that New is reducible first *)
+        iModIntro. iSplit.
+        - iPureIntro; unfold base_reducible; repeat eexists; eapply NewS.
+        (* need to show that we can summon a fresh location *)
+        exact (is_fresh s1).
+        - (* now we need to handle the state update, 
+            first bring variables into scope  *)
+        iModIntro. iIntros (e2 s2 efs baseStep) "lc".
+        (* inversion on the base step *)
+        inversion baseStep; subst ; simpl.
+        (*  Show that we can extend state s1 with a fresh location *)
+        assert (s1 ~~> (s1 ∪ {[l]})) as update by done.
+        (* now how do we use that update to modify name_set 
+            using own_update? 
+          first, we only need the ownership under the update modality
+            so use the frame rules to shove things around  
+        *)
+        iApply fupd_frame_l.
+        iSplit. { done. }
+        iApply fupd_frame_r.
+        (* here we need to make a choice w.r.t. the spacial context
+           We dont need HPhi to prove ownership, but we do need it to show
+           that the post condition holds, so push it to that goal  *)
+        iSplitL "HStinterp".
+        (* now we can update the name_set *)
+        {
+            iMod (own_update name_set s1 _ update with "HStinterp");
+            iModIntro ; done. 
+        }
+        rewrite H2. done.
+    Qed.
+ *)
+
+
+
+End lang_rules.
+
+
+
+
+
